\documentclass[a4paper,12pt]{article}
\usepackage[landscape]{geometry}
\begin{document}

\section{2-D FTCS}

\begin{equation}
T_{a,b}^{\theta+1} = T_{a,b}^{\theta} + C \left(T_{a+1,b}^{\theta}
+ T_{a-1,b}^{\theta} - 4T_{a,b}^{\theta} + T_{a,b-1}^{\theta}
+ T_{a,b+1}^{\theta} \right)
\end{equation}

\begin{equation}
T_{a,b}^{\theta} = G^n e^{-ika\Delta x} e^{-ilb\Delta x}
\end{equation}

Substituting (2) into (1) and simplifying...

\[
\frac{G^{n+1}}{G^n} = 1 + C
\left(
e^{ik\Delta x} + e^{-ik\Delta x}
+ e^{il\Delta x} + e^{-il\Delta x}
- 4
\right)
\]

\[
\frac{G^{n+1}}{G^n} = 1 + C
\left(
2cos(k \Delta x) + 2cos(l \Delta x) -  4
\right)
\]

\[
-1 \leq 1 - 8C \leq 1
\]

\[
-2 \leq - 8C \leq 0
\]

\[
0 \leq C \leq \frac{1}{4}
\]

\pagebreak
\section{3-D FTCS}

\begin{equation}
T_{a,b,c}^{\theta+1} = T_{a,b,c}^{\theta} + C \left(
T_{a+1,b,c}^{\theta}
+ T_{a-1,b,c}^{\theta}
+ T_{a,b+1,c}^{\theta}
+T_{a,b-1,c}^{\theta}
+T_{a,b,c+1}^{\theta}
+T_{a,b,c-1}^{\theta}
- 6T_{a,b,c}^{\theta}
\right)
\end{equation}

\begin{equation}
T_{a,b}^{\theta} = G^n e^{-ika\Delta x} e^{-ilb\Delta x} e^{-imc\Delta x}
\end{equation}

Substituting (4) into (3) and simplifying...

\[
\frac{G^{n+1}}{G^n} = 1 + C
\left(
e^{ik\Delta x} + e^{-ik\Delta x}
+ e^{il\Delta x} + e^{-il\Delta x}
+ e^{im\Delta x} + e^{-im\Delta x}
- 6
\right)
\]

\[
\frac{G^{n+1}}{G^n} = 1 + C
\left(
2cos(k \Delta x) + 2cos(l \Delta x) + 2cos(m \Delta x)- 6
\right)
\]

\[
-1 \leq 1 - 12C \leq 1
\]

\[
-2 \leq - 12C \leq 0
\]

\[
0 \leq C \leq \frac{1}{6}
\]

\pagebreak
\section{1-D BECS}

\begin{equation}
T_{a}^{\theta+1} = T_{a}^{\theta} + C \left(T_{a+1,b}^{\theta+1}
- 2T_{a}^{\theta+1}
+ T_{a-1}^{\theta+1}
\right)
\end{equation}

\begin{equation}
T_{a}^{\theta} = G^n e^{-ika\Delta x}
\end{equation}

Substituting (6) into (5) and simplifying...

\[
G^{n+1} = G^n + C G^{n+1}
\left(
e^{ik\Delta x} + e^{-ik\Delta x}
- 2
\right)
\]

\[
\frac{G^n}{G^{n+1}} = 1 - C
\left(
2cos(k \Delta x) -  2
\right)
\]

\[
\frac{G^{n+1}}{G^n} = \frac{1}{1 - C
\left(
2cos(k \Delta x) -  2
\right)}
\]

\[
-1 \leq \frac{1}{1 + 4C} \leq 1
\]

\[
-1-4C \leq 1 \leq 1+4C
\]

\[
-1 \leq 2C \leq 4C
\]

BECS is unconditionally stable, since C is unbounded.

\pagebreak
\section{2-D BECS}

\begin{equation}
T_{a,b}^{\theta+1} = T_{a,b}^{\theta} + C \left(
T_{a+1,b}^{\theta+1}
T_{a,b+1}^{\theta+1}
- 4T_{a,b}^{\theta+1}
+ T_{a-1,b}^{\theta+1}
T_{a,b-1}^{\theta+1}
\right)
\end{equation}

\begin{equation}
T_{a,b}^{\theta} = G^n e^{-ika\Delta x} e^{-ilb\Delta x}
\end{equation}

Substituting (8) into (7) and simplifying...

\[
G^{n+1} = G^n + C G^{n+1}
\left(
e^{ik\Delta x} + e^{-ik\Delta x}
e^{il\Delta x} + e^{-il\Delta x}
- 4
\right)
\]

\[
\frac{G^n}{G^{n+1}} = 1 + C
\left(
2cos(k \Delta x) + 2cos(l \Delta x) -  4
\right)
\]

\[
\frac{G^{n+1}}{G^n} = \frac{1}{1 + C
\left(
2cos(k \Delta x) + 2cos(l \Delta x) -  4
\right)}
\]

\[
-1 \leq \frac{1}{1 + 8C} \leq 1
\]

\[
-1-8C \leq 1 \leq 1+8C
\]

\[
-1 \leq 4C \leq 8C
\]

BECS is unconditionally stable, since C is unbounded.

\pagebreak
\section{3-D BECS}

\begin{equation}
T_{a,b,c}^{\theta+1} = T_{a,b,c}^{\theta} + C \left(
T_{a+1,b,c}^{\theta+1}
T_{a,b+1,c}^{\theta+1}
T_{a,b,c+1}^{\theta+1}
- 6T_{a,b,c}^{\theta+1}
+ T_{a-1,b,c}^{\theta+1}
T_{a,b-1,c}^{\theta+1}
T_{a,b,c-1}^{\theta+1}
\right)
\end{equation}

\begin{equation}
T_{a,b,c}^{\theta} = G^n e^{-ika\Delta x} e^{-ilb\Delta x}e^{-imb\Delta x}
\end{equation}

Substituting (10) into (9) and simplifying...

\[
G^{n+1} = G^n + C G^{n+1}
\left(
e^{ik\Delta x} + e^{-ik\Delta x}
e^{il\Delta x} + e^{-il\Delta x}
e^{im\Delta x} + e^{-im\Delta x}
- 6
\right)
\]

\[
\frac{G^n}{G^{n+1}} = 1 + C
\left(
2cos(k \Delta x) + 2cos(l \Delta x) + 2cos(m \Delta x) - 6
\right)
\]

\[
\frac{G^{n+1}}{G^n} = \frac{1}{1 + C
\left(
2cos(k \Delta x) + 2cos(l \Delta x) + 2cos(m \Delta x) -  6
\right)}
\]

\[
-1 \leq \frac{1}{1 + 12C} \leq 1
\]

\[
-1-12C \leq 1 \leq 1+12C
\]

\[
-1 \leq 6C \leq 12C
\]

BECS is unconditionally stable, since C is unbounded.

\pagebreak
\section{1-D Crank-Nicolson}

\begin{equation}
T_{a}^{\theta+1} = T_{a}^{\theta} + \frac{C}{2} \left(
T_{a+1,b}^{\theta+1}
- 2T_{a}^{\theta+1}
+ T_{a-1}^{\theta+1}
+ T_{a+1,b}^{\theta}
- 2T_{a}^{\theta}
+ T_{a-1}^{\theta}
\right)
\end{equation}

\begin{equation}
T_{a}^{\theta} = G^n e^{-ika\Delta x}
\end{equation}

Substituting (12) into (11) and simplifying...

\section{2-D Crank-Nicolson}

\section{3-D Crank-Nicolson}


\end{document}
